src/lowparse/pulse/LowParse.Pulse.VCList.fst
@@ -2,7 +2,7 @@ module LowParse.Pulse.VCList
 include LowParse.Spec.VCList
 include LowParse.Pulse.Combinators
 open FStar.Tactics.V2
-open LowParse.Pulse.Util
+open Pulse.Lib.Pervasives open Pulse.Lib.Slice.Util open Pulse.Lib.Trade
 open Pulse.Lib.Slice
 
 module SZ = FStar.SizeT
